backend/StackingproofC1.v
@@ -1,0 +1,348 @@
+Require Import CoqlibC Errors.
+Require Import Integers ASTC Linking.
+Require Import ValuesC Memory Separation Events GlobalenvsC Smallstep.
+Require Import LTL Op Locations LinearC MachC.
+Require Import Bounds Conventions Stacklayout Lineartyping.
+Require Import Stacking.
+
+Local Open Scope sep_scope.
+
+(* newly added *)
+Require Import sflib.
+Require Export StackingproofC0.
+Require Import SimModSem.
+Require Import SimMemInj.
+Require SimSymb.
+Require Import Asmregs.
+
+Set Implicit Arguments.
+
+
+
+
+
+Section ALIGN.
+
+  Lemma align_refl
+        x
+        (NONNEG: x >= 0)
+  :
+    <<ALIGN: align x x = x>>
+  .
+  Proof.
+    destruct (Z.eqb x 0) eqn: T.
+    { rewrite Z.eqb_eq in T. clarify. }
+    rewrite Z.eqb_neq in T.
+    red.
+    unfold align.
+    replace ((x + x - 1) / x) with 1.
+    { xomega. }
+    replace (x + x - 1) with (1 * x + (1 * x + (- 1))); cycle 1.
+    { xomega. }
+    rewrite Z.div_add_l; try eassumption.
+    rewrite Z.div_add_l; try eassumption.
+    replace (Z.div (Zneg xH) x) with (Zneg xH).
+    { xomega. }
+    destruct x; ss.
+    clear - p.
+    unfold Z.div. des_ifs.
+    ginduction p; i; ss; des_ifs.
+  Qed.
+
+  Lemma align_zero
+        x
+    :
+      <<ALIGN: align x 0 = 0>>
+  .
+  Proof.
+    unfold align. red. ss.
+    xomega.
+  Qed.
+
+  Lemma align_divisible
+        z y
+        (DIV: (y | z))
+        (NONNEG: y > 0)
+    :
+      <<ALIGN: align z y = z>>
+  .
+  Proof.
+    red.
+    unfold align.
+    replace ((z + y - 1) / y) with (z / y + (y - 1) / y); cycle 1.
+    {
+      unfold Z.divide in *. des. clarify.
+      rewrite Z_div_mult; ss.
+      replace (z0 * y + y - 1) with (z0 * y + (y - 1)); cycle 1.
+      { xomega. }
+      rewrite Z.div_add_l with (b := y); ss.
+      xomega.
+    }
+    replace ((y - 1) / y) with 0; cycle 1.
+    { erewrite Zdiv_small; ss. xomega. }
+    unfold Z.divide in *. des. clarify.
+    rewrite Z_div_mult; ss.
+    rewrite Z.add_0_r.
+    xomega.
+  Qed.
+
+  Lemma align_idempotence
+        x y
+        (NONNEG: y > 0)
+    :
+      <<ALIGN: align (align x y) y = align x y>>
+  .
+  Proof.
+    apply align_divisible; ss.
+    apply align_divides; ss.
+  Qed.
+
+End ALIGN.
+
+Hint Rewrite align_refl: align.
+Hint Rewrite align_zero: align.
+Hint Rewrite align_idempotence: align.
+
+
+
+
+
+Section DUMMY_FUNCTION.
+
+  Variable sg: signature.
+  
+  Lemma dummy_function_used_callee_save
+    :
+    (dummy_function sg).(function_bounds).(used_callee_save) = []
+  .
+  Proof. ss. Qed.
+
+  Lemma dummy_function_bound_local
+    :
+      (dummy_function sg).(function_bounds).(bound_local) = 0
+  .
+  Proof. ss. Qed.
+
+  Lemma dummy_function_bound_outgoing
+    :
+      (dummy_function sg).(function_bounds).(bound_outgoing) = (size_arguments sg)
+  .
+  Proof.
+    ss. unfold dummy_function. cbn.
+    rewrite Z.max_l; try xomega. rewrite Z.max_r; try xomega.
+    generalize (size_arguments_above sg). i. xomega.
+  Qed.
+
+  Lemma dummy_function_bound_stack_data
+    :
+      (dummy_function sg).(function_bounds).(bound_stack_data) = 0
+  .
+  Proof. ss. Qed.
+
+  Lemma dummy_function_size_callee_save_area
+        ofs
+    :
+      (dummy_function sg).(function_bounds).(size_callee_save_area) ofs = ofs
+  .
+  Proof. ss. Qed.
+
+  Hint Rewrite dummy_function_size_callee_save_area: dummy.
+
+  Lemma dummy_function_fe_size
+    :
+      (dummy_function sg).(function_bounds).(make_env).(fe_size) = 0
+  .
+  Proof.
+    unfold make_env.
+    (*??????????????? simpl. -> inf loop, but cbn works!!!!!!!!!!!!! *)
+    cbn. des_ifs_safe. rewrite Z.max_l; try xomega. rewrite Z.max_r; cycle 1.
+    { generalize (size_arguments_above sg). i. xomega. }
+    autorewrite with align. des_ifs.
+  Abort.
+
+End DUMMY_FUNCTION.
+
+Hint Rewrite dummy_function_used_callee_save: dummy.
+Hint Rewrite dummy_function_bound_local: dummy.
+Hint Rewrite dummy_function_bound_outgoing: dummy.
+Hint Rewrite dummy_function_bound_stack_data: dummy.
+Hint Rewrite dummy_function_size_callee_save_area: dummy.
+
+Local Opaque Z.add Z.mul Z.div.
+
+
+Print typesize.
+Print loc_arguments_64. (* always + 2 *)
+(* Lemma size_arguments_loc_arguments_64 *)
+(*       x tys ir fr *)
+(*       (SIZE: 0 <= x < 4 * size_arguments_64 tys ir fr 0) *)
+(*   : *)
+(*     exists sl pos ty, In (S sl pos ty) (loc_arguments_64 tys ir fr 0).(regs_of_rpairs) *)
+(* . *)
+(* Proof. *)
+(*   ginduction tys; ii; ss. *)
+(*   { xomega. } *)
+(*   destruct a; ss. *)
+(*   - des_ifs. *)
+(*     + esplits; eauto. *)
+(* Qed. *)
+
+(* Lemma size_arguments_loc_arguments *)
+(*       ofs sg *)
+(*       (SIZE: 0 <= ofs < 4 * size_arguments sg) *)
+(*   : *)
+(*     exists sl pos ty, In (S sl pos ty) (loc_arguments sg).(regs_of_rpairs) *)
+(* . *)
+(* Proof. *)
+(*   destruct sg; ss. unfold size_arguments in *. unfold loc_arguments in *. des_ifs_safe. ss. clear_tac. *)
+(*   ginduction sig_args; ii; ss. *)
+(*   { xomega. } *)
+(* Qed. *)
+
+Section PRESERVATION.
+
+Local Existing Instance Val.mi_normal.
+Context `{SimSymbId: @SimSymb.SimSymb.class SimMemInj}.
+Variable prog: Linear.program.
+Variable tprog: Mach.program.
+Hypothesis TRANSF: match_prog prog tprog.
+Variable return_address_offset: function -> code -> ptrofs -> Prop.
+Let match_states := match_states prog tprog return_address_offset.
+
+Definition msp: ModSemPair.t :=
+  ModSemPair.mk (LinearC.modsem prog) (MachC.modsem return_address_offset tprog) (admit "simsymb") Nat.lt.
+
+Local Transparent dummy_stack.
+
+Ltac sep_split := econs; [|split]; swap 2 3.
+Hint Unfold fe_ofs_arg.
+ 
+Theorem init_match_states
+        (sm_init: SimMem.SimMem.t) fptr_init_src fptr_init_tgt
+        (FPTRREL: Val.inject (inj sm_init) fptr_init_src fptr_init_tgt)
+        rs_init_src rs_init_tgt
+        (RSREL: SimMem.SimMem.sim_regset sm_init rs_init_src rs_init_tgt)
+        (WF: wf' sm_init)
+        (SIMSKENV: ModSemPair.sim_skenv msp sm_init)
+        st_init_src
+        (INITSRC: LinearC.initial_frame prog rs_init_src sm_init.(src_mem) st_init_src)
+  :
+    exists st_init_tgt,
+      <<INITTGT: initial_frame rs_init_tgt (tgt_mem sm_init) st_init_tgt>>
+                               /\ <<MATCH: match_states st_init_src st_init_tgt>>
+.
+Proof.
+  ss. u in *. unfold ModSemPair.sim_skenv in *. ss. clear SIMSKENV.
+  inv INITSRC.
+  esplits; eauto.
+  - econs; eauto.
+  -
+    assert(PTRRSP: is_real_fptr (rs_init_tgt RSP)).
+    { admit "corollary of sem.". }
+    assert(PTRRA: is_real_ptr (rs_init_tgt RA)).
+    { admit "add to sem". }
+
+    econs; eauto.
+    + instantiate (1:= sm_init.(inj)).
+      u in *. des_ifs.
+      generalize (Ptrofs.eq_spec i0 Ptrofs.zero). i; des_ifs. clarify. clear_tac.
+      econs; eauto.
+      i.
+      assert(ACC: loc_argument_acceptable (S Outgoing ofs ty)).
+      { eapply loc_arguments_acceptable_2; eauto. }
+      assert(VALID: slot_valid (dummy_function (Linear.fn_sig fd)) Outgoing ofs ty).
+      { destruct ACC. unfold slot_valid, proj_sumbool.
+        rewrite zle_true by omega. rewrite pred_dec_true by auto. reflexivity. }
+      {
+        intros; red.
+          eapply Z.le_trans with (size_arguments _); eauto.
+          apply loc_arguments_bounded; eauto.
+        u.
+        xomega.
+      }
+    + ii.
+      u in RSREL.
+      Hint Unfold SimMem.SimMem.sim_regset. (* TODO: move to proper place *)
+      u in RSREL. u.
+      Hint Unfold mregset_of.
+      u.
+      inv LOCSET.
+      rewrite <- REGS.
+      eapply RSREL.
+    + ii. des_ifs.
+    + eapply RSREL.
+    +
+      {
+        Local Opaque sepconj.
+        simpl. des_ifs.
+        u in PTRRA. des_ifs. u in PTRRSP. des_ifs.
+        generalize (Ptrofs.eq_spec i Ptrofs.zero). i; des_ifs. clarify. clear_tac.
+
+        rewrite sep_assoc. rewrite sep_comm. rewrite sep_assoc.
+        rewrite sep_pure. split; ss.
+        rewrite sep_assoc.
+        rewrite sep_comm.
+        rewrite sep_assoc.
+        sep_split.
+        { simpl. esplits; eauto. admit "SimSymbId". admit "SimSymbId". }
+        { ii. ss. }
+        rewrite sep_comm.
+        sep_split.
+        { simpl. apply WF. }
+        { ii. admit "raw admit. footprint". }
+        unfold frame_contents.
+        econs.
+        - sep_split.
+          { unfold make_env in *.
+            autorewrite with dummy.
+            des_ifs. cbn.
+            esplits; eauto.
+            - apply align_divides. xomega.
+            - admit "easy".
+            - rewrite Z.mul_0_r. rewrite Z.add_0_r.
+              About size_no_overflow.
+              admit "[SIZE]
+1) transf_function is succeeded -> size is somehow bound.
+2) worst case, add to sem.".
+            -
+              (* Print Hint *. *)
+              (* Print HintDb typeclass_instances. *)
+              Fail autorewrite with zarith. (* TODO *)
+              rewrite Z.mul_0_r. rewrite Z.add_0_r.
+              ii. des. xomega.
+            - ii.
+              generalize (typesize_pos ty). i. xomega.
+          }
+          { cbn. des_ifs.
+            ii. ss. des. clarify.
+Local Transparent sepconj.
+            ss. des; ss; clarify; clear_tac; try xomega.
+Local Opaque sepconj.
+          }
+
+          sep_split.
+          { autorewrite with dummy.
+            ss.
+            esplits; eauto; u; try xomega.
+            - apply Z.divide_0_r.
+            - admit "[SIZE] ditto.".
+            - rewrite Z.add_0_l. ii.
+              inv LOCSET.
+          }
+        -
+      }
+Qed.
+
+Theorem sim
+  :
+    ModSemPair.sim msp
+.
+Proof.
+  econs; eauto.
+  { admit "garbage". }
+  ii.
+  ss.
+  split; ss.
+Qed.
+
+End PRESERVATION.
