common/ValuesC.v
@@ -1,0 +1,42 @@
+(* *********************************************************************)
+(*                                                                     *)
+(*              The Compcert verified compiler                         *)
+(*                                                                     *)
+(*          Xavier Leroy, INRIA Paris-Rocquencourt                     *)
+(*                                                                     *)
+(*  Copyright Institut National de Recherche en Informatique et en     *)
+(*  Automatique.  All rights reserved.  This file is distributed       *)
+(*  under the terms of the GNU General Public License as published by  *)
+(*  the Free Software Foundation, either version 2 of the License, or  *)
+(*  (at your option) any later version.  This file is also distributed *)
+(*  under the terms of the INRIA Non-Commercial License Agreement.     *)
+(*                                                                     *)
+(* *********************************************************************)
+
+(** This module defines the type of values that is used in the dynamic
+  semantics of all our intermediate languages. *)
+
+Require Import CoqlibC.
+Require Import AST.
+Require Import Integers.
+Require Import Floats.
+Require Import sflib.
+(** newly added **)
+Require Export Values.
+
+Definition is_real_ptr (v: val): bool :=
+  match v with
+  | Vptr _ _ true => true
+  | _ => false
+  end
+.
+Hint Unfold is_real_ptr.
+
+Definition is_real_fptr (v: val): bool :=
+  match v with
+  | Vptr _ ofs true => if (Ptrofs.eq ofs Ptrofs.zero) then true else false
+  | _ => false
+  end
+.
+Hint Unfold is_real_fptr.
+
